matching-logic/src/DerivedOperators_Semantics.v
@@ -1,7 +1,4 @@
 From Coq Require Import ssreflect ssrfun ssrbool.
-Set Implicit Arguments.
-Unset Strict Implicit.
-Unset Printing Implicit Defensive.
 
 Require Setoid.
 From stdpp Require Import base sets propset.
