matching-logic/src/SyntaxLemmas/ApplicationCtxSubstitution.v
@@ -1,7 +1,4 @@
 From Coq Require Import ssreflect ssrfun ssrbool.
-Set Implicit Arguments.
-Unset Strict Implicit.
-Unset Printing Implicit Defensive.
 
 From stdpp Require Import base tactics sets.
 
